starting to doubt that IterationT is worth it

Iterator/Basic.lean
@@ -127,11 +127,19 @@ theorem IterStep.map_id {it : IterStep α β} :
   simp only [map]
   cases it <;> simp
 
+theorem IterStep.map_id' {it : IterStep α β} :
+    it.map (·) (·) = it :=
+  map_id
+
 theorem IterStep.map_map {α' : Type u'} {β' : Type v'} {f : α → α'} {g : β → β'}
     {α'' : Type u''} {β'' : Type v''} {f' : α' → α''} {g' : β' → β''} {it : IterStep α β} :
     (it.map f g).map f' g' = it.map (f · |> f') (g · |> g') := by
   simp only [map]
   cases it <;> simp
+
+theorem IterStep.successor_map {α' : Type u'} {β' : Type v'} {f : α → α'} {g : β → β'} {step : IterStep α β} :
+    (step.map f g).successor = step.successor.elim none (some <| f ·) := by
+  cases step <;> rfl
 
 def PlausibleIterStep (plausible_step : IterStep α β → Prop) := Subtype plausible_step
 
@@ -179,80 +187,199 @@ theorem PlausibleIterStep.map_id {plausible_step : IterStep α β → Prop}
 --   -- cases it <;> simp
 
 class Iterator (α : Type u) (m : Type w → Type w') (β : outParam (Type v)) where
-  stepInternal : IterationT m (IterStep α β)
+  step : α → IterationT m (IterStep α β)
 
-abbrev PlausibleIterStep.for {α β} (m) [Iterator α m β] (it : α) :=
-  PlausibleIterStep (Iterator.plausible_step m it)
+-- abbrev PlausibleIterStep.for {α β} (m) [Iterator α m β] (it : α) :=
+--   PlausibleIterStep (Iterator.plausible_step m it)
 
-abbrev PlausibleIterStep.liftedFor {α β} (m) [Iterator α m β] (it : α) [ComputableSmall.{w} α] [ComputableSmall.{w} β] : Type w :=
-  PlausibleIterStep
-    (fun step => Iterator.plausible_step m it <| step.map ComputableSmall.down ComputableSmall.down)
+-- abbrev PlausibleIterStep.liftedFor {α β} (m) [Iterator α m β] (it : α) [ComputableSmall.{w} α] [ComputableSmall.{w} β] : Type w :=
+--   PlausibleIterStep
+--     (fun step => Iterator.plausible_step m it <| step.map ComputableSmall.down ComputableSmall.down)
 
-@[always_inline, inline]
-def PlausibleIterStep.up {α β m} [Iterator α m β] [ComputableSmall.{w} α] [ComputableSmall.{w} β]
-    {it : α} (step : PlausibleIterStep.for m it) : PlausibleIterStep.liftedFor m it :=
-  match step with
-  | .yield it' b h => .yield (ComputableSmall.up it') (ComputableSmall.up b) (by simp [IterStep.map, ComputableSmall.down_up, h])
-  | .skip it' h => .skip (ComputableSmall.up it') (by simp [IterStep.map, ComputableSmall.down_up, h])
-  | .done h => .done h
+-- @[always_inline, inline]
+-- def PlausibleIterStep.up {α β m} [Iterator α m β] [ComputableSmall.{w} α] [ComputableSmall.{w} β]
+--     {it : α} (step : PlausibleIterStep.for m it) : PlausibleIterStep.liftedFor m it :=
+--   match step with
+--   | .yield it' b h => .yield (ComputableSmall.up it') (ComputableSmall.up b) (by simp [IterStep.map, ComputableSmall.down_up, h])
+--   | .skip it' h => .skip (ComputableSmall.up it') (by simp [IterStep.map, ComputableSmall.down_up, h])
+--   | .done h => .done h
 
-@[always_inline, inline]
-def PlausibleIterStep.down {α β m} [Iterator α m β] {_ : ComputableSmall.{w} α} {_ : ComputableSmall.{w} β} {it : α}
-    (step : PlausibleIterStep.liftedFor m it) : PlausibleIterStep.for m it :=
-  match step with
-  | .yield it' b h => .yield (ComputableSmall.down it') (ComputableSmall.down b) h
-  | .skip it' h => .skip (ComputableSmall.down it') h
-  | .done h => .done h
+-- @[always_inline, inline]
+-- def PlausibleIterStep.down {α β m} [Iterator α m β] {_ : ComputableSmall.{w} α} {_ : ComputableSmall.{w} β} {it : α}
+--     (step : PlausibleIterStep.liftedFor m it) : PlausibleIterStep.for m it :=
+--   match step with
+--   | .yield it' b h => .yield (ComputableSmall.down it') (ComputableSmall.down b) h
+--   | .skip it' h => .skip (ComputableSmall.down it') h
+--   | .done h => .done h
 
 section Finite
 
-structure FiniteIteratorWF (α m) [Iterator α m β] where
-  inner : α
-
-def FiniteIteratorWF.lt {α m β} [Iterator α m β] (x y : FiniteIteratorWF α m) : Prop :=
-  (∃ b, Iterator.plausible_step m y.inner (.yield x.inner b)) ∨
-    Iterator.plausible_step m y.inner (.skip x.inner)
-
-def finiteIteratorWF {α m β} [Iterator α m β] (it : α) : FiniteIteratorWF α m :=
-  ⟨it⟩
+def Iterator.successor_of {α β} (m) [Iterator α m β] (x y : α) : Prop :=
+  Iterator.step (m := m) y |>.mapH IterStep.successor |>.property (some x)
+  -- (∃ b, Iterator.plausible_step m y.inner (.yield x.inner b)) ∨
+  --   Iterator.plausible_step m y.inner (.skip x.inner)
 
 class Finite (α m) [Iterator α m β] : Prop where
-  wf : WellFounded (FiniteIteratorWF.lt (α := α) (m := m))
+  wf : WellFounded (Iterator.successor_of (α := α) m)
 
-instance [Iterator α m β] [Finite α m] : WellFoundedRelation (FiniteIteratorWF α m) where
-  rel := FiniteIteratorWF.lt
-  wf := Finite.wf
+theorem Iterator.successor_of_yield {α m β} [Iterator α m β] {x y : α} {out : β}
+    (h : Iterator.step (m := m) y |>.property (.yield x out)) : Iterator.successor_of m x y :=
+  ⟨_, rfl, h⟩
 
-macro_rules | `(tactic| decreasing_trivial) => `(tactic| first | exact Or.inl ⟨_, ‹_›⟩ | exact Or.inr ‹_›)
+theorem Iterator.successor_of_skip {α m β} [Iterator α m β] {x y : α}
+    (h : Iterator.step (m := m) y |>.property (.skip x)) : Iterator.successor_of m x y :=
+  ⟨_, rfl, h⟩
 
 end Finite
 
 section Productive
 
-structure ProductiveIteratorWF (α m) [Iterator α m β] where
-  inner : α
-
-def ProductiveIteratorWF.lt {α m β} [Iterator α m β] (x y : ProductiveIteratorWF α m) : Prop :=
-  Iterator.plausible_step m y.inner (.skip x.inner)
-
-def productiveIteratorWF {α m β} [Iterator α m β] (it : α) : ProductiveIteratorWF α m :=
-  ⟨it⟩
+def Iterator.skip_successor_of {α β} (m) [Iterator α m β] (x y : α) : Prop :=
+  Iterator.step (m := m) y |>.property (.skip x)
 
 class Productive (α m) [Iterator α m β] : Prop where
-  wf : WellFounded (ProductiveIteratorWF.lt (α := α) (m := m))
-
-instance {m} [Iterator α m β] [Productive α m] : WellFoundedRelation (ProductiveIteratorWF α m) where
-  rel := ProductiveIteratorWF.lt
-  wf := Productive.wf
-
-theorem ProductiveIteratorWF.subrelation_finiteIteratorWF {α m β} [Iterator α m β] :
-    Subrelation (α := ProductiveIteratorWF α m)
-      ProductiveIteratorWF.lt
-      (InvImage FiniteIteratorWF.lt (finiteIteratorWF (m := m) ∘ inner)) := by
-  intro x y
-  exact Or.inr
-
-instance {m} [Iterator α m β] [Finite α m] : Productive α m where
-  wf := ProductiveIteratorWF.subrelation_finiteIteratorWF.wf (InvImage.wf _ Finite.wf)
+  wf : WellFounded (Iterator.skip_successor_of (α := α) m)
 
 end Productive
+
+variable (α m) in
+class FinitenessRelation [Iterator α m β] where
+  rel : α → α → Prop
+  wf : WellFounded rel
+  subrelation : {it it' : α} → ((Iterator.step (m := m) it).mapH IterStep.successor).property (some it') → rel it' it
+
+variable (α m) in
+class ProductivenessRelation [Iterator α m β] where
+  rel : α → α → Prop
+  wf : WellFounded rel
+  subrelation : {it it' : α} → (Iterator.step (m := m) it).property (.skip it') → rel it' it
+
+instance [Iterator α m β] [FinitenessRelation α m] : Finite α m where
+  wf := by
+    refine Subrelation.wf (r := FinitenessRelation.rel (m := m) β) ?_ ?_
+    · intro x y h
+      apply FinitenessRelation.subrelation
+      exact h
+    · apply InvImage.wf
+      exact FinitenessRelation.wf
+
+instance [Iterator α m β] [ProductivenessRelation α m] : Productive α m where
+  wf := by
+    refine Subrelation.wf (r := ProductivenessRelation.rel (m := m) β) ?_ ?_
+    · intro x y h
+      apply ProductivenessRelation.subrelation
+      exact h
+    · apply InvImage.wf
+      exact ProductivenessRelation.wf
+
+def matchStep {α β γ} (yield : α → β → γ) (skip : α → γ) (done : γ) (step : IterStep α β) : γ :=
+  match step with
+  | .yield it out => yield it out
+  | .skip it => skip it
+  | .done => done
+
+-- def matchStepD {α β γ} (step : IterStep α β)
+--     (yield : (it : α) → (out : β) → step = .yield it out → γ)
+--     (skip : (it : α) → step = .skip it → γ) (done : step = .done → γ) : γ :=
+--   match step with
+--   | .yield it out => yield it out rfl
+--   | .skip it => skip it rfl
+--   | .done => done rfl
+
+theorem apply_matchStep {α β γ δ} (f : γ → δ) {yield : α → β → γ} {skip : α → γ} {done : γ} {step : IterStep α β} :
+    f (matchStep yield skip done step) = matchStep (yield · · |> f) (skip · |> f) (f done) step := by
+  cases step <;> rfl
+
+def matchStepComputation {m α β γ} (yield : α → β → IterationT m γ) (skip : α → IterationT m γ) (done : IterationT m γ) (step : IterStep α β) :
+    CodensityT m (matchStep yield skip done step).Plausible :=
+      match step with
+      | .yield it out => (yield it out).computation
+      | .skip it => (skip it).computation
+      | .done => done.computation
+
+def matchStepD {α β} {motive : IterStep α β → Type v}
+    (yield : (it : α) → (out : β) → motive (.yield it out))
+    (skip : (it : α) → motive (.skip it))
+    (done : motive .done) (step : IterStep α β) :
+    motive step :=
+      match step with
+      | .yield it out => (yield it out)
+      | .skip it => (skip it)
+      | .done => done
+
+def matchStepComputation' {m α β γ} (yield : α → β → IterationT m γ) (skip : α → IterationT m γ) (done : IterationT m γ) (step : IterStep α β) :
+    CodensityT m (matchStep yield skip done step).Plausible :=
+      matchStepD (motive := fun step => CodensityT m (matchStep yield skip done step |>.Plausible))
+        (yield · · |>.computation)
+        (skip · |>.computation)
+        done.computation
+        step
+
+theorem computation_matchStep {m α β γ} {yield : α → β → IterationT m γ} {skip : α → IterationT m γ} {done : IterationT m γ} {step : IterStep α β} :
+    (matchStep yield skip done step).computation =
+      matchStepD (motive := fun step => CodensityT m (matchStep yield skip done step |>.Plausible))
+        (yield · · |>.computation)
+        (skip · |>.computation)
+        done.computation
+        step := by
+  cases step <;> rfl
+
+theorem apply_matchStepD {α β} {motive : IterStep α β → Type v}
+    {motive' : IterStep α β → Type v'}
+    (yield : (it : α) → (out : β) → motive (.yield it out))
+    (skip : (it : α) → motive (.skip it))
+    (done : motive .done) (step : IterStep α β)
+    {f : {step : IterStep α β} → motive step → motive' step} :
+    f (matchStepD yield skip done step) =
+      sorry := sorry
+
+inductive MatchStepVerificationCases {α : Type u} {m : Type w → Type w'} {β : Type v} {γ : Type x}
+    [Iterator α m β] (it : α) (yield : α → β → IterationT m γ) (skip : α → IterationT m γ)
+    (done : IterationT m γ) (x : γ) : Prop where
+  | yield {it' : α} {out : β} :
+    (Iterator.step (m := m) it).property (.yield it' out) →
+    (yield it' out).property x → MatchStepVerificationCases it yield skip done x
+  | skip {it' : α} :
+    (Iterator.step (m := m) it).property (.skip it') →
+    (skip it').property x → MatchStepVerificationCases it yield skip done x
+  | done :
+    (Iterator.step (m := m) it).property .done →
+    done.property x → MatchStepVerificationCases it yield skip done x
+
+theorem successor_matchStepH {α : Type u} {m : Type w → Type w'} {β : Type v} {γ : Type x} {δ : Type y}
+    [Iterator α m β]
+    {it : α} {yield skip done}
+    {f : γ → δ} {x : δ}
+    (h : (IterationT.mapH f <| (Iterator.step (m := m) it).bindH <| matchStep (γ := IterationT m γ) yield skip done).property x) :
+    MatchStepVerificationCases it (yield · · |>.mapH f) (skip · |>.mapH f) (done.mapH f) x := by
+  simp only [IterationT.mapH, IterationT.bindH, matchStep] at h
+  obtain ⟨c, rfl, _, h, h'⟩ := h
+  split at h
+  · exact .yield h' ⟨c, rfl, h⟩
+  · exact .skip h' ⟨c, rfl, h⟩
+  · exact .done h' ⟨c, rfl, h⟩
+
+theorem successor_yield [Pure m] [Iterator α m β] {it₁ it₂ : α} {b : β} :
+    ((pure (.yield it₁ b) : IterationT m (IterStep α β)).mapH IterStep.successor).property (some it₂) ↔
+      it₂ = it₁ := by
+  simp [IterationT.mapH, Pure.pure, IterStep.successor]
+
+theorem successor_skip [Pure m] [Iterator α m β] {it₁ it₂ : α} :
+    ((pure (.skip it₁) : IterationT m (IterStep α β)).mapH IterStep.successor).property (some it₂) ↔
+      it₂ = it₁ := by
+  simp [IterationT.mapH, Pure.pure, IterStep.successor]
+
+theorem successor_done [Pure m] [Iterator α m β] {it: α} :
+    ((pure .done : IterationT m (IterStep α β)).mapH IterStep.successor).property (some it) ↔ False := by
+  simp [IterationT.mapH, Pure.pure, IterStep.successor]
+
+theorem property_matchStepH {α : Type u} {m : Type w → Type w'} {β : Type v} {γ : Type x}
+    [Iterator α m β] {it : α} {yield skip done} {x : γ}
+    (h : (Iterator.step (m := m) it |>.bindH <| matchStep (γ := IterationT m γ) yield skip done).property x) :
+    MatchStepVerificationCases it yield skip done x := by
+  simp only [IterationT.bindH, matchStep] at h
+  obtain ⟨c, h, h'⟩ := h
+  split at h
+  · exact .yield h' h
+  · exact .skip h' h
+  · exact .done h' h
