Iterator/IterationT.lean
@@ -13,6 +13,22 @@ structure IterationT (m : Type w → Type w') (γ : Type u) where
   property : γ → Prop
   computation : CodensityT m { c : γ // property c }
 
+def IterationT.Plausible {m : Type w → Type w'} {γ : Type u} (x : IterationT m γ) : Type u :=
+  { c : γ // x.property c }
+
+def IterationT.Plausible.copy {m : Type w → Type w'} {γ : Type u} {s t : IterationT m γ} (h : s = t)
+    (x : s.Plausible) : t.Plausible :=
+  ⟨x.1, h ▸ x.2⟩
+
+def IterationT.Plausible.copy_rfl {m : Type w → Type w'} {γ : Type u} {s : IterationT m γ}
+    {x : s.Plausible} :
+    x.copy rfl = x := rfl
+
+theorem plausible_eq_copy {m : Type w → Type w'} {γ : Type u} {s t : IterationT m γ} (h : s = t) :
+    s.computation = (IterationT.Plausible.copy h.symm ·) <$> t.computation := by
+  cases h
+  simp  [IterationT.Plausible.copy_rfl, CodensityT.map_eq_mapH, CodensityT.mapH_id']
+
 instance : Monad (IterationT m) where
   pure a := { property b := (b = a)
               computation := pure ⟨a, rfl⟩ }
@@ -36,18 +52,70 @@ def IterationT.liftWithProperty {p : γ → Prop} (t : CodensityT m { c : γ // 
   { property := p, computation := t }
 
 @[always_inline, inline]
-def IterationT.mapH {γ : Type u} {m : Type w → Type w'} [Monad m]
+def IterationT.mapH {γ : Type u} {m : Type w → Type w'}
     {δ : Type v}
     (f : γ → δ)
     (t : IterationT m γ) : IterationT m δ :=
   { property d := ∃ c, d = f c ∧ t.property c,
     computation := t.computation.mapH fun c => ⟨f c.1, c.1, rfl, c.2⟩ }
 
+theorem IterationT.map_eq_mapH {γ δ : Type u} {m : Type w → Type w'} {f : γ → δ} {t : IterationT m γ} :
+    f <$> t = t.mapH f := rfl
+
+theorem IterationT.mapH_id {γ : Type u} {m : Type w → Type w'} {t : IterationT m γ} :
+    t.mapH id = t := by
+  simp only [mapH, id]
+  let prop d := ∃ c, d = c ∧ t.property c
+  have : prop = t.property := by
+    ext c
+    exact ⟨fun ⟨_, rfl, h⟩ => h, fun h => ⟨c, rfl, h⟩⟩
+  let trafo (p : { p : γ → Prop // p = t.property }) : IterationT m γ :=
+    { property := p.1
+      computation := t.computation.mapH (fun x => ⟨x.val, by rw [p.2]; exact x.2⟩) }
+  exact (congrArg trafo (Subtype.eq_iff.mpr this : ⟨prop, this⟩ = ⟨t.property, rfl⟩))
+
+theorem IterationT.mapH_id' {γ : Type u} {m : Type w → Type w'} {t : IterationT m γ} :
+    t.mapH (·) = t :=
+  IterationT.mapH_id
+
+theorem IterationT.mapH_mapH {γ : Type u} {δ : Type u'} {ε : Type u''} {m : Type w → Type w'}
+    {f : γ → δ} {g : δ → ε} {t : IterationT m γ} :
+    (t.mapH f).mapH g = t.mapH (f · |> g) := by
+  simp only [mapH, CodensityT.mapH_mapH]
+  let prop d := ∃ c, d = g (f c) ∧ t.property c
+  let prop' d := ∃ c, d = g c ∧ ∃ c', c = f c' ∧ t.property c'
+  have : prop = prop' := by
+    ext y
+    simp only [prop, prop']
+    apply Iff.intro
+    · rintro ⟨c, rfl, h⟩
+      exact ⟨f c, rfl, c, rfl, h⟩
+    · rintro ⟨c, rfl, c', rfl, h⟩
+      exact ⟨c', rfl, h⟩
+  let trafo (p : { p : ε → Prop // p = prop }) : IterationT m ε :=
+    { property := p.1
+      computation := t.computation.mapH (fun x => ⟨(g (f x.val)), by rw [p.2]; exact ⟨x.1, rfl, x.2⟩⟩) }
+  have := congrArg trafo (Subtype.eq_iff.mpr this : ⟨prop, rfl⟩ = ⟨prop', this.symm⟩)
+  refine this.symm.trans ?_
+  simp [trafo, prop]
+
+theorem IterationT.property_mapH {γ : Type u} {δ : Type u'} {m : Type w → Type w'} {t : IterationT m γ}
+    {x : γ} (f : γ → δ) (h : t.property x) : (t.mapH f).property (f x) :=
+  ⟨x, rfl, h⟩
+
+def IterationT.Plausible.map {m : Type w → Type w'} {γ : Type u} {δ : Type u'}
+    {t : IterationT m γ} (f : γ → δ) (x : t.Plausible) : (t.mapH f).Plausible :=
+  ⟨f x.1, x.1, rfl, x.2⟩
+
 @[always_inline, inline]
-def IterationT.bindH {m : Type w → Type w'} [Monad m] {γ : Type u} {δ : Type v}
+def IterationT.bindH {m : Type w → Type w'} {γ : Type u} {δ : Type v}
     (t : IterationT m γ) (f : γ → IterationT m δ) : IterationT m δ :=
   { property d := ∃ c, (f c).property d ∧ t.property c
     computation := t.computation.bindH fun c => (f c.1).computation.mapH fun d => ⟨d.1, c.1, d.2, c.2⟩}
+
+theorem IterationT.mapH_eq_bindH {γ : Type u} {δ : Type u'} {m : Type w → Type w'} {f : γ → δ}
+    {t : IterationT m γ} :
+    t.mapH f = t.bindH (pure <| f ·) := rfl
 
 @[always_inline, inline]
 def IterationT.liftInnerMonad {γ : Type w} {m : Type w → Type w'} [Pure m] (n : Type w → Type w'') [Monad n] [MonadLift m n] (t : IterationT m γ) :
