Iterator/Wrapper.lean
@@ -4,6 +4,7 @@ Released under Apache 2.0 license as described in the file LICENSE.
 Authors: Paul Reichert
 -/
 prelude
+import Init.Data.Option.Lemmas
 import Iterator.Basic
 import Iterator.Cont
 
@@ -27,9 +28,38 @@ theorem inner_toIter {_ : Iterator α m β} {_ : ComputableSmall.{w} α} (it : �
     (toIter m it).inner = it :=
   ComputableSmall.down_up
 
+def Iterator.stepLift [Iterator α m β] [ComputableSmall.{w} α] [ComputableSmall.{w} β] (it : α) :
+    IterationT m (IterStep (ComputableSmall.Lift α) (ComputableSmall.Lift β)) :=
+  Iterator.step (m := m) it |>.mapH (·.map ComputableSmall.up ComputableSmall.up)
+
+def Iterator.stepLiftState [Iterator α m β] [ComputableSmall.{w} α] (it : α) :
+    IterationT m (IterStep (ComputableSmall.Lift α) β) :=
+  Iterator.step (m := m) it |>.mapH (·.map ComputableSmall.up id)
+
+def Iter.plausible_step {_ : Iterator α m β} {_ : ComputableSmall.{w} α} (it : Iter (α := α) m β)
+    (step : IterStep (Iter (α := α) m β) β) : Prop :=
+  Iterator.step (m := m) it.inner |>.mapH (·.map (toIter m) id) |>.property step
+
 def Iter.Step {_ : Iterator α m β} {_ : ComputableSmall.{w} α} (it : Iter (α := α) m β) :=
-  PlausibleIterStep (α := Iter (α := α) m β)
-    (fun step => Iterator.plausible_step m it.inner <| step.map Iter.inner id)
+  { step : IterStep (Iter (α := α) m β) β // it.plausible_step step }
+  -- Iterator.step (m := m) it.inner |>.mapH (·.map (toIter m) id) |>.Plausible
+
+def Iter.Step.toPlausible {_ : Iterator α m β} {_ : ComputableSmall.{w} α} {it : Iter (α := α) m β}
+    (step : Iter.Step it) :
+    Iterator.step (m := m) it.inner |>.mapH (·.map (toIter m) id) |>.Plausible :=
+  step
+
+@[match_pattern]
+def Iter.Step.yield {_ : Iterator α m β} {_ : ComputableSmall.{w} α}
+   {it : Iter (α := α) m β} (it' b h) := (⟨.yield it' b, h⟩ : it.Step)
+
+@[match_pattern]
+def Iter.Step.skip {_ : Iterator α m β} {_ : ComputableSmall.{w} α}
+   {it : Iter (α := α) m β} (it' h) := (⟨.skip it', h⟩ : it.Step)
+
+@[match_pattern]
+def Iter.Step.done {_ : Iterator α m β} {_ : ComputableSmall.{w} α}
+   {it : Iter (α := α) m β} (h) := (⟨.done, h⟩ : it.Step)
 
 -- inductive Iter.Step {_ : Iterator α m β} {_ : ComputableSmall.{w} α} (it : Iter (α := α) m β) where
 -- | yield : (it' : Iter (α := α) m β) → (b : β) → Iterator.yielded m it.inner it'.inner b → it.Step
@@ -38,8 +68,19 @@ def Iter.Step {_ : Iterator α m β} {_ : ComputableSmall.{w} α} (it : Iter (α
 
 def Iter.LiftedStep {_ : Iterator α m β} {_ : ComputableSmall.{w} α} [ComputableSmall.{w} β]
    (it : Iter (α := α) m β) : Type w :=
-  PlausibleIterStep (α := Iter (α := α) m β)
-    (fun step => Iterator.plausible_step m it.inner <| step.map Iter.inner ComputableSmall.down)
+  Iterator.step (m := m) it.inner |>.mapH (·.map (fun x => toIter m x) ComputableSmall.up) |>.Plausible
+
+@[match_pattern]
+def Iter.LiftedStep.yield {_ : Iterator α m β} {_ : ComputableSmall.{w} α} [ComputableSmall.{w} β]
+   {it : Iter (α := α) m β} (it' b h) := (⟨.yield it' b, h⟩ : it.LiftedStep)
+
+@[match_pattern]
+def Iter.LiftedStep.skip {_ : Iterator α m β} {_ : ComputableSmall.{w} α} [ComputableSmall.{w} β]
+   {it : Iter (α := α) m β} (it' h) := (⟨.skip it', h⟩ : it.LiftedStep)
+
+@[match_pattern]
+def Iter.LiftedStep.done {_ : Iterator α m β} {_ : ComputableSmall.{w} α} [ComputableSmall.{w} β]
+   {it : Iter (α := α) m β} (h) := (⟨.done, h⟩ : it.LiftedStep)
 
 -- inductive Iter.LiftedStep {_ : Iterator α m β} {_ : ComputableSmall.{w} α} [ComputableSmall.{w} β]
 --     (it : Iter (α := α) m β) where
@@ -49,28 +90,20 @@ def Iter.LiftedStep {_ : Iterator α m β} {_ : ComputableSmall.{w} α} [Computa
 
 @[always_inline, inline]
 def Iter.Step.lift {_ : Iterator α m β} {_ : ComputableSmall.{w} α} [ComputableSmall.{w} β]
-    (it : Iter (α := α) m β) (step : it.Step) : it.LiftedStep :=
-  step.map id ComputableSmall.up _
-    (by intro _ h; simp only [IterStep.map_map, ComputableSmall.down_up]; exact h)
-  -- match step with
-  -- | .yield it' b h => .yield it' (ComputableSmall.up b) (by simp [ComputableSmall.down_up, h])
-  -- | .skip it' h => .skip it' h
-  -- | .done h => .done h
+    (it : Iter (α := α) m β) (step : it.Step) : it.LiftedStep := by
+  refine step.toPlausible.map (fun s => s.map id ComputableSmall.up) |>.copy ?_
+  simp [Iterator.stepLift, Iterator.stepLiftState, IterationT.mapH_mapH, IterStep.map_map]
 
 @[always_inline, inline]
-def Iter.Step.ofInternal {_ : Iterator α m β} {_ : ComputableSmall.{w} α} (it : Iter (α := α) m β) (step : PlausibleIterStep.for m it.inner) :
-    it.Step :=
-  step.map  (toIter m) id _
-    (by intro _ h; simp only [IterStep.map_map, inner_toIter]; exact IterStep.map_id ▸ h)
-  -- match step with
-  -- | .yield it' b h => .yield (toIter m it') b (by simp only [inner_toIter, h])
-  -- | .skip it' h => .skip (toIter m it') (by simp only [inner_toIter, h])
-  -- | .done h => .done h
+def Iter.Step.ofInternal {_ : Iterator α m β} {_ : ComputableSmall.{w} α} (it : Iter (α := α) m β) (step : Iterator.step (m := m) it.inner |>.Plausible) :
+    it.Step := by
+  exact step.map _
 
 @[always_inline, inline]
 def Iter.Step.toInternal {_ : Iterator α m β} {_ : ComputableSmall.{w} α} (it : Iter (α := α) m β) (step : it.Step) :
-    PlausibleIterStep.for m it.inner :=
-  step.map Iter.inner id _ (by simp)
+    Iterator.step (m := m) it.inner |>.Plausible := by
+  refine step.toPlausible.map (fun s => s.map Iter.inner id) |>.copy ?_
+  simp only [IterationT.mapH_mapH, inner_toIter, IterStep.map_map, id_eq, IterStep.map_id', IterationT.mapH_id']
 
 -- instance {m} [Functor m] [Iterator α m β] : Iterator (Iter (α := α) m β) m β where
 --   yielded it it' b := Iterator.yielded m it.inner it'.inner b
@@ -91,14 +124,103 @@ def Iter.Step.toInternal {_ : Iterator α m β} {_ : ComputableSmall.{w} α} (it
 @[always_inline, inline]
 def Iter.stepH [Monad m] {_ : Iterator α m β} {_ : ComputableSmall.{w} α} (it : Iter (α := α) m β) :
     CodensityT m it.Step :=
-  Iterator.step it.inner |>.mapH (Iter.Step.ofInternal it)
+  Iterator.step it.inner |>.computation |>.mapH (Iter.Step.ofInternal it)
 
 @[always_inline, inline]
 def Iter.step {β : Type w} [Monad m] {_ : Iterator α m β} {_ : ComputableSmall.{w} α} (it : Iter (α := α) m β) :
     m (Iter.Step it) :=
   it.stepH.run
 
+section Finite
+
+structure Iter.FiniteWFRel (α : Type u) (m : Type w → Type w') [Iterator α m β] where
+  inner : α
+
 @[always_inline, inline]
 def Iter.terminationByFinite {_ : Iterator α m β} {_ : ComputableSmall.{w} α} [Finite α m] (it : Iter (α := α) m β) :
-    FiniteIteratorWF α m :=
-  finiteIteratorWF it.inner
+    Iter.FiniteWFRel α m :=
+  ⟨it.inner⟩
+
+def Iter.FiniteWFRel.rel [Iterator α m β] [Finite α m] : FiniteWFRel α m → FiniteWFRel α m → Prop :=
+  InvImage (Iterator.successor_of m) Iter.FiniteWFRel.inner
+
+instance [Iterator α m β] [Finite α m] : WellFoundedRelation (Iter.FiniteWFRel α m) where
+  rel := Iter.FiniteWFRel.rel
+  wf := InvImage.wf _ Finite.wf
+
+private theorem Option.elim_elim {α : Type u} {β : Type v} {γ : Type w} (o : Option α)
+    {d₁ : Option β} {f₁ : α → Option β} {d₂ : γ} {f₂ : β → γ} :
+    (o.elim d₁ f₁).elim d₂ f₂ = o.elim (d₁.elim d₂ f₂) (f₁ . |>.elim d₂ f₂) := by
+  cases o <;> rfl
+
+private theorem Option.elim_id {α : Type u} (o : Option α) :
+    o.elim none (some ·) = o := by
+  cases o <;> rfl
+
+def Iter.FiniteWFRel.of_step_yield {α m β} {_ : Iterator α m β} [Finite α m] {_ : ComputableSmall.{w} α}
+    {it' it : Iter (α := α) m β} {out : β} (h : (Iterator.step (m := m) it.inner).mapH (·.map (toIter m) id) |>.property (.yield it' out)) : Iter.FiniteWFRel.rel it'.terminationByFinite it.terminationByFinite := by
+  simp_wf
+  simp [Iter.FiniteWFRel.rel, Iterator.successor_of]
+  refine ⟨.yield it'.inner out, rfl, ?_⟩
+  have h' : (Iterator.step (m := m) it.inner).mapH (·.map (toIter m) id) |>.mapH (·.map Iter.inner id) |>.property (.yield it'.inner out) :=
+    ⟨_, rfl, h⟩
+  simpa only [IterationT.mapH_mapH, IterStep.map_map, inner_toIter, id_eq, IterStep.map_id', IterationT.mapH_id'] using h'
+
+def Iter.FiniteWFRel.of_step_skip {α m β} {_ : Iterator α m β} [Finite α m] {_ : ComputableSmall.{w} α}
+    {it' it : Iter (α := α) m β} (h : (Iterator.step (m := m) it.inner).mapH (·.map (toIter m) id) |>.property (.skip it')) : Iter.FiniteWFRel.rel it'.terminationByFinite it.terminationByFinite := by
+  simp_wf
+  simp [Iter.FiniteWFRel.rel, Iterator.successor_of]
+  refine ⟨.skip it'.inner, rfl, ?_⟩
+  have h' : (Iterator.step (m := m) it.inner).mapH (·.map (toIter m) id) |>.mapH (·.map Iter.inner id) |>.property (.skip it'.inner) :=
+    ⟨_, rfl, h⟩
+  simpa only [IterationT.mapH_mapH, IterStep.map_map, inner_toIter, id_eq, IterStep.map_id', IterationT.mapH_id'] using h'
+
+def Iter.FiniteWFRel.of_stepH_yield {α m β} {_ : Iterator α m β} [Finite α m]
+    {_ : ComputableSmall.{w} α} {_ : ComputableSmall.{w} β}
+    {it' it : Iter (α := α) m β} {out : ComputableSmall.Lift β}
+    (h : (Iterator.step (m := m) it.inner).mapH (·.map (toIter m) ComputableSmall.up) |>.property (.yield it' out)) :
+    Iter.FiniteWFRel.rel it'.terminationByFinite it.terminationByFinite := by
+  apply Iter.FiniteWFRel.of_step_yield
+  simpa [IterationT.mapH_mapH, IterStep.map_map, ComputableSmall.down_up] using
+    IterationT.property_mapH (·.map id ComputableSmall.down) h
+
+def Iter.FiniteWFRel.of_stepH_skip {α m β} {_ : Iterator α m β} [Finite α m]
+    {_ : ComputableSmall.{w} α} {_ : ComputableSmall.{w} β}
+    {it' it : Iter (α := α) m β}
+    (h : (Iterator.step (m := m) it.inner).mapH (·.map (toIter m) ComputableSmall.up) |>.property (.skip it')) :
+    Iter.FiniteWFRel.rel it'.terminationByFinite it.terminationByFinite := by
+  apply Iter.FiniteWFRel.of_step_skip
+  simpa [IterationT.mapH_mapH, IterStep.map_map, ComputableSmall.down_up] using
+    IterationT.property_mapH (·.map id ComputableSmall.down) h
+
+macro_rules | `(tactic| decreasing_trivial) => `(tactic|
+  first
+  | exact Iter.FiniteWFRel.of_step_yield ‹_›
+  | exact Iter.FiniteWFRel.of_step_skip ‹_›
+  | exact Iter.FiniteWFRel.of_stepH_yield ‹_›
+  | exact Iter.FiniteWFRel.of_stepH_skip ‹_›)
+
+end Finite
+
+-- section Productive
+
+-- structure ProductiveIteratorWF (α m) [Iterator α m β] where
+--   inner : α
+
+-- def productiveIteratorWF {α m β} [Iterator α m β] (it : α) : ProductiveIteratorWF α m :=
+--   ⟨it⟩
+
+-- instance {m} [Iterator α m β] [Productive α m] : WellFoundedRelation (ProductiveIteratorWF α m) where
+--   rel := ProductiveIteratorWF.lt
+--   wf := Productive.wf
+
+-- theorem ProductiveIteratorWF.subrelation_finiteIteratorWF {α m β} [Iterator α m β] :
+--     Subrelation (α := ProductiveIteratorWF α m)
+--       ProductiveIteratorWF.lt
+--       (InvImage FiniteIteratorWF.lt (finiteIteratorWF (m := m) ∘ inner)) :=
+--   fun h => FiniteIteratorWF.lt_of_skip h
+
+-- instance {m} [Iterator α m β] [Finite α m] : Productive α m where
+--   wf := ProductiveIteratorWF.subrelation_finiteIteratorWF.wf (InvImage.wf _ Finite.wf)
+
+-- end Productive
