Iterator/Proofs.lean
@@ -1,71 +1,163 @@
-import Iterator
+import Iterator.Combinators.FilterMap
 
-section Equivalence
+-- section Equivalence
 
-variable {α : Type u} {m : Type w → Type w'} {β : Type v}
+-- variable {α : Type u} {m : Type w → Type w'} {β : Type v}
 
-inductive IterTStep (β : Type v) where
-  | yield : β → IterTStep β
-  | skip : IterTStep β
-  | done : IterTStep β
+-- inductive IterTStep (β : Type v) where
+--   | yield : β → IterTStep β
+--   | skip : IterTStep β
+--   | done : IterTStep β
 
-inductive IterT (m : Type w → Type w') (β : Type v) : Type w → Type (max v w w' + 1) where
-  | step : ∀ {α}, Nat → (β → α) → IterT m β (IterTStep α)
-  | lift : ∀ {α}, m α → IterT m β α
-  | bind : ∀ {α γ}, IterT m β α → (α → IterT m β γ) → IterT m β γ
+-- inductive IterT (m : Type w → Type w') (β : Type v) : Type w → Type (max v w w' + 1) where
+--   | step : ∀ {α}, Nat → (β → α) → IterT m β (IterTStep α)
+--   | lift : ∀ {α}, m α → IterT m β α
+--   | bind : ∀ {α γ}, IterT m β α → (α → IterT m β γ) → IterT m β γ
 
-def IterT.interpret [Iterator α m β] [Monad m] (it : α) (γ : Type w) (x : IterT m β γ) : m γ :=
-  go [it] x |>.mapH (fun p => p.1) |>.run
-where
-  go {δ : Type w} (its : List α) : IterT m β δ → CodensityT m (δ × List α)
-    | .step n f => match its[n]? with
-      | none => pure (.done, its)
-      | some it =>
-        let v := Iterator.step it
-        v.mapH (match · with
-          | .yield it' out _ => (.yield (f out), it' :: its)
-          | .skip it' _ => (.skip, it' :: its)
-          | .done _ => (.done, its))
-    | .lift x => (CodensityT.eval x).mapH (Prod.mk · its)
-    | .bind x f => (go its x) >>= (fun y => go y.2 (f y.1))
+-- def IterT.interpret [Iterator α m β] [Monad m] (it : α) (γ : Type w) (x : IterT m β γ) : m γ :=
+--   go [it] x |>.mapH (fun p => p.1) |>.run
+-- where
+--   go {δ : Type w} (its : List α) : IterT m β δ → CodensityT m (δ × List α)
+--     | .step n f => match its[n]? with
+--       | none => pure (.done, its)
+--       | some it =>
+--         let v := Iterator.step it
+--         v.mapH (match · with
+--           | .yield it' out _ => (.yield (f out), it' :: its)
+--           | .skip it' _ => (.skip, it' :: its)
+--           | .done _ => (.done, its))
+--     | .lift x => (CodensityT.eval x).mapH (Prod.mk · its)
+--     | .bind x f => (go its x) >>= (fun y => go y.2 (f y.1))
 
-end Equivalence
+-- end Equivalence
 
 variable {α : Type u} {m : Type w → Type w'} {β : Type v}
   [Iterator α m β] {_ : ComputableSmall.{w} α} (it : Iter (α := α) m β)
-  [Monad m] [LawfulMonad m]
+  [Monad m]
   (f : β → CodensityT m (Option β'))
 
-theorem filterMapMH_step' (it : α) (f : β → IterationT m (Option β')) :
-    Iterator.step (m := m) (Iterator.filterMapMH f it) =
-      (Iterator.step (m := m) it |>.bindH (match · with
-        | .yield it' out h => (f out).computation.mapH (fun x => ⟨match x.val with
-          | none => .skip ⟨it'⟩
-          | some out => .yield ⟨it'⟩ out, .yield it' out, ⟨x.1, rfl, x.2⟩, h⟩)
-        | .skip it' h => pure ⟨.skip ⟨it'⟩, .skip it', rfl, h⟩
-        | .done h => pure ⟨.done, .done, rfl, h⟩)) := by
-  simp [Iterator.filterMapMH, Iterator.step, SimpleIterator.step, computation_matchStepH,
-    IterationT.step, IterationT.mapH, CodensityT.mapH_mapH, IterationT.computation_pure]
-  refine congrArg (CodensityT.bindH _) ?_
-  ext x
-  split
-  · simp
-    refine congrArg (CodensityT.mapH · _) ?_
-    ext y
-    cases y
-    dsimp only
-    split <;> rfl
-  · simp
+-- theorem filterMapMH_step' (it : α) (f : β → IterationT m (Option β')) :
+--     Iterator.step (m := m) (Iterator.filterMapMH f it) =
+--       (Iterator.step (m := m) it |>.bindH (match · with
+--         | .yield it' out h => (f out).computation.mapH (fun x => ⟨match x.val with
+--           | none => .skip ⟨it'⟩
+--           | some out => .yield ⟨it'⟩ out, .yield it' out, ⟨x.1, rfl, x.2⟩, h⟩)
+--         | .skip it' h => pure ⟨.skip ⟨it'⟩, .skip it', rfl, h⟩
+--         | .done h => pure ⟨.done, .done, rfl, h⟩)) := by
+--   simp [Iterator.filterMapMH, Iterator.step, SimpleIterator.step, computation_matchStepH,
+--     IterationT.step, IterationT.mapH, CodensityT.mapH_mapH, IterationT.computation_pure]
+--   refine congrArg (CodensityT.bindH _) ?_
+--   ext x
+--   split
+--   · simp
+--     refine congrArg (CodensityT.mapH · _) ?_
+--     ext y
+--     cases y
+--     dsimp only
+--     split <;> rfl
+--   · simp
+
+theorem FilterMapMH.plausible_of_yield_of_none {it' : Iter (α := α) m β} {out : β}
+    (h : it.plausible_step (.yield it' out)) :
+    (it.filterMapMH f).plausible_step (.skip (it'.filterMapMH f)) := by
+  let step : it.Step := .yield it' out h
+  let internalStep := step.toInternal
+  simp only [Iter.plausible_step]
+  refine ⟨.skip (it'.filterMapMH f).inner, by simp [IterStep.map, Iter.filterMapMH], ?_⟩
+  refine ⟨.yield (it'.filterMapMH f).inner.inner out, ?_, ?_⟩
+  · exact ⟨none, rfl, True.intro⟩
+  · simp only [Iter.filterMapMH, Iterator.filterMapMH, inner_toIter]
+    exact internalStep.property
+
+theorem FilterMapMH.plausible_of_yield_of_some {it' : Iter (α := α) m β} {out : β} {out' : β'}
+    (h : it.plausible_step (.yield it' out)) :
+    (it.filterMapMH f).plausible_step (.yield (it'.filterMapMH f) out') := by
+  let step : it.Step := .yield it' out h
+  let internalStep := step.toInternal
+  refine ⟨.yield (it'.filterMapMH f).inner out', by simp [IterStep.map, Iter.filterMapMH], ?_⟩
+  refine ⟨.yield (it'.filterMapMH f).inner.inner out, ?_, ?_⟩
+  · exact ⟨some out', rfl, True.intro⟩
+  · simp only [Iter.filterMapMH, Iterator.filterMapMH, inner_toIter]
+    exact internalStep.property
+
+theorem FilterMapMH.plausible_of_skip {it' : Iter (α := α) m β}
+    (h : it.plausible_step (.skip it')) :
+    (it.filterMapMH f).plausible_step (.skip (it'.filterMapMH f)) := by
+  let step : it.Step := .skip it' h
+  let internalStep := step.toInternal
+  refine ⟨.skip (it'.filterMapMH f).inner, by simp [IterStep.map, Iter.filterMapMH], ?_⟩
+  refine ⟨.skip (it'.filterMapMH f).inner.inner, rfl, ?_⟩
+  simp only [Iter.filterMapMH, Iterator.filterMapMH, inner_toIter]
+  exact internalStep.property
+
+theorem FilterMapMH.plausible_of_done
+    (h : it.plausible_step .done) :
+    (it.filterMapMH f).plausible_step .done := by
+  let step : it.Step := .done h
+  let internalStep := step.toInternal
+  refine ⟨.done, by simp [IterStep.map, Iter.filterMapMH], ?_⟩
+  refine ⟨.done, rfl, ?_⟩
+  simp only [Iter.filterMapMH, Iterator.filterMapMH, inner_toIter]
+  exact internalStep.property
 
 theorem filterMapMH_step :
   (it.filterMapMH f).stepH = (it.stepH.bindH (match · with
       | .yield it' out h => (f out).mapH fun
-          | none => .skip (it'.filterMapMH f) ⟨sorry, sorry⟩
-          | _ => sorry
-      | .skip it' h => pure <| .skip (it'.filterMapMH f) sorry
-      | .done h => pure <| .done sorry)) := by
+          | none => .skip (it'.filterMapMH f) (FilterMapMH.plausible_of_yield_of_none _ _ h)
+          | some out' => .yield (it'.filterMapMH f) out' (FilterMapMH.plausible_of_yield_of_some _ _ h)
+      | .skip it' h => pure <| .skip (it'.filterMapMH f) (FilterMapMH.plausible_of_skip _ _ h)
+      | .done h => pure <| .done (FilterMapMH.plausible_of_done _ _ h))) := by
+  cases it
+  simp only [Iter.filterMapMH, Iterator.filterMapMH]
+  rw [Iter.stepH, CodensityT.mapH_eq_bindH]
+  rw [Iter.stepH, CodensityT.mapH_eq_bindH]
+  simp only [plausible_eq_copy
+    (congrArg Iterator.step (inner_toIter ..)),
+    congrArg Iterator.step, congrArg FilterMapMH.inner, inner_toIter]
+  simp only [Iterator.step]
+  rw [CodensityT.map_eq_mapH, CodensityT.mapH_eq_bindH]
+  simp only [IterationT.bindH]
+  simp only [CodensityT.bindH_assoc]
+  refine congrArg (CodensityT.bindH _ ·) ?_
+  ext x
+  simp only [CodensityT.bindH_pure, Iter.Step.ofInternal, IterationT.Plausible.map, IterStep.map]
+  match h : x with
+  | ⟨.yield .., h⟩ =>
+    simp only [matchStep]
+    simp only [IterationT.mapH, CodensityT.mapH_eq_bindH, monadLift, MonadLift.monadLift,
+      CodensityT.map_eq_mapH, CodensityT.mapH_eq_bindH, CodensityT.bindH_assoc,
+      CodensityT.bindH_pure]
+    refine congrArg (CodensityT.bindH _ ·) ?_
+    ext y
+    refine congrArg pure ?_
+    simp only [IterationT.Plausible.copy, Iter.Step.yield, Iter.Step.skip, Iter.filterMapMH,
+      Iterator.filterMapMH, inner_toIter]
+    cases y <;> rfl
+  | ⟨.skip .., h⟩ =>
+    simp only [matchStep]
+    simp only [CodensityT.mapH_eq_bindH, IterationT.computation_pure, CodensityT.bindH_pure,
+      IterationT.Plausible.copy, Iter.Step.skip, Iter.filterMapMH, Iterator.filterMapMH,
+      inner_toIter]
+  | ⟨.done, h⟩ =>
+    simp only [matchStep, IterationT.Plausible.copy, CodensityT.mapH_eq_bindH, CodensityT.bindH_assoc,
+      IterationT.computation_pure, CodensityT.bindH_pure]
+    rfl
+
+#exit
+  simp only [plausible_eq_copy
+    (congrArg Iterator.step (inner_toIter ..)),
+    congrArg Iterator.step, congrArg FilterMapMH.inner, inner_toIter]
+
+  simp [Iter.filterMapH, Iter.stepH, Iterator.step]
   simp [Iter.filterMapMH, Iter.stepH]
+  simp [IterationT.bindH, IterationT.mapH]
+  simp only [plausible_eq_copy
+    (congrArg (Iterator.step (m := m) (α := α))
+      (congrArg FilterMapMH.inner (inner_toIter ..))),
+    congrArg Iterator.step, congrArg FilterMapMH.inner, inner_toIter]
+  simp [Iterator.filterMapMH]
   simp [toIter, Iter.inner]
+  simp [computation_matchStep, IterationT.computation_pure]
   rw [Iterator.step_congr <| ComputableSmall.down_up ..]
   rw [filterMapMH_step']
   simp [CodensityT.map_eq_mapH, CodensityT.mapH_mapH]
